added a field in function to indicate it is a drop glue or not

rustfrontend/Dropglue.ml
@@ -36,6 +36,6 @@ let create_union_idents (a: positive) : (positive * positive) * positive =
 
 let malloc_id =
   intern_string "malloc"
-
+  
 let free_id =
   intern_string "free"
