rustfrontend/ElaborateDrop.v
@@ -343,6 +343,7 @@ Definition transf_function (ce: composite_env) (f: function) : Errors.res functi
           let stmt' := transl_stmt (snd st.(gen_map)) st.(gen_stmt) in
           Errors.OK (mkfunction f.(fn_generic_origins)
                                 f.(fn_origins_relation)
+                                f.(fn_drop_glue)
                         f.(fn_return)
                         f.(fn_callconv)                        
                         (f.(fn_vars) ++ st.(gen_trail))
@@ -370,7 +371,6 @@ Definition transl_program (p: program) : Errors.res program :=
               prog_public := AST.prog_public p1;
               prog_main := AST.prog_main p1;
               prog_types := prog_types p;
-              prog_drop_glue := prog_drop_glue p;
               prog_comp_env := prog_comp_env p;
               prog_comp_env_eq := prog_comp_env_eq p |}.
 
