Makefile
@@ -171,7 +171,7 @@ RUSTFRONTENT=Rusttypes.v Rustsyntax.v RustlightBase.v RustIR.v\
   InitAnalysis.v ElaborateDrop.v\
   BorrowCheckDomain.v ReplaceOrigins.v BorrowCheckPolonius.v\
   Clightgen.v Clightgenspec.v Clightgenproof.v\
-  RustOp.v Rusttyping.v
+  RustOp.v
 
 # Parser
 
